ContractEnv.thy
@@ -1,9 +1,9 @@
 section {* Some Data Types for EVM *}
 
-text {* This development depends on Isabelle/HOL's machine word library. *}
-text {* The machine word library is one of the biggest reasons for choosing Isabelle/HOL
-for this development. *}
-text {* The Ethereum Virtual Machine depends on 8-bit bytes and 256-bit machine words. *}
+text {* This development depends on Isabelle/HOL's machine word library.
+The machine word library is one of the biggest reasons for choosing Isabelle/HOL
+for this development.
+The Ethereum Virtual Machine depends on 8-bit bytes and 256-bit machine words. *}
 
 theory ContractEnv
 
@@ -11,8 +11,9 @@ imports Main "~~/src/HOL/Word/Word"
 
 begin
 
-text {* Frequently used machine words are named here.  For example, address denotes the type of
-160-bit machine words.  The type uint denotes the type of EVM machine words. *}
+text {* The frequently used machine words are named here.  For example, ``address''
+denotes the type of
+160-bit machine words.  The type ``uint'' denotes the type of EVM machine words. *}
 
 type_synonym uint = "256 word"    -- {* 256 bit words *}
 type_synonym address = "160 word" -- {* 160 bit addresses *}
@@ -62,21 +63,21 @@ record aenv =
   aenv_value_sent :: uint -- {* The amount of Eth sent alont the current invocation. *}
   aenv_data_sent :: "byte list" -- {* The data sent along the current invocation. *}
   aenv_storage_at_call :: storage -- {* The storage content at the time of the invocation. *}
-  aenv_balance_at_call :: "address \<Rightarrow> uint" -- {* The balance of all accounts at the time of the
-  invocation *}
+  aenv_balance_at_call :: "address \<Rightarrow> uint"
+  -- {* The balance of all accounts at the time of the invocation *}
   aenv_this :: address -- {* The address of this contract under verification. *}
-  aenv_origin :: address -- {* The original external account that started the whole transaction. *}
+  aenv_origin :: address -- {* The external account that started the transaction. *}
 
-text {* The @{term aenv_balance} keeps track of the balance of all accounts because the contract
-under verification sends some Eth to other accounts.  To capture the effect of this, I chose to
+text {* @{term aenv_balance} field keeps track of the balance of all accounts because the contract
+under verification can send some Eth to other accounts.  To capture the effect of this, I chose to
 keep track of the balances of the other contracts.  *}
 
-text {* @{term aenv_storage_at_call} and @{term aenv_balance_at_call} keep the states at the
-time of the contract invocation.  These are used for rollback after a failure.
-The contract under verification might fail
-when it jumps to a wrong destination, or it runs out of gas. *}
+text {* @{term aenv_storage_at_call} and @{term aenv_balance_at_call} fields keep the states at the
+time of the contract invocation.  These are used for rolling back the state after a failure.
+Failures happen for example when the contract under verification jumps to a wrong destination,
+or it runs out of gas. *}
 
-text {* @{term aenv_origin} might be the same but might be different from @{term aenv_caller}.
+text {* @{term aenv_origin} might be the same as but might be different from @{term aenv_caller}.
 An Ethereum transaction is started by an external account (that is, an account which does not
 have codes but owned by somebody with a secret key).  @{term aenv_origin} denotes this external
 account.  During a transaction, the origin first sends a message to an account, the receiver can
@@ -84,6 +85,7 @@ in turn call other accounts as well.  When the calls nest, @{term aenv_caller} p
 immediate caller.
 *}
 
-text {* I'm going to add more fields in the @{typ aenv} record in the near future. *}
+text {* I'm going to add more fields in the @{typ aenv} record in the near future because
+it does not contain all the information available at the execution time. *}
   
 end
